Valaig/Aig/Lemmas.lean
@@ -4,3 +4,4 @@ public import Valaig.Aig.Lemmas.Basic
 public import Valaig.Aig.Lemmas.Modify
 public import Valaig.Aig.Lemmas.Monotone
 public import Valaig.Aig.Lemmas.WellFormed
+public import Valaig.Aig.Lemmas.Iter
