Valaig/Aig/Lemmas/Iter.lean
@@ -1,0 +1,321 @@
+module
+
+import all Valaig.Aig.Basic
+public import Valaig.Aig.Basic
+import Valaig.Aig.Lemmas.Monotone
+import Valaig.Aig.Lemmas.Basic
+import Valaig.Utils.GrindIter
+import Init.Data.Iterators.Lemmas.Basic
+
+public section
+namespace Valaig.Aig
+variable {aig : Aig}
+
+/-
+  `iter`/`iterVal`/`iterEnd`.
+-/
+
+section iter
+namespace VarIter
+
+variable {m : Type -> Type _} [Pure m]
+
+attribute [local ext, local grind ext] Std.Iter Std.IterM VarIter
+attribute [local grind] Std.Iter.toIterM step iterVal iterEnd
+attribute [local grind =] IsPlausibleStep_iff IsPlausibleSuccessorOf_iff
+
+variable {it it' : @Std.Iter aig.VarIter Var}
+
+@[simp, grind .]
+theorem IsPlausibleStep_skip:
+    ¬it.IsPlausibleStep (.skip it') := by
+  grind
+
+@[simp, grind norm]
+theorem step_eq_IsPlausibleStep {step} :
+    it.step.val = step ↔ it.IsPlausibleStep step := by
+  grind
+
+@[local simp, local grind =]
+private theorem iterVal_eq :
+    aig.iterVal it = it.internalState.var := by
+  grind
+
+@[local grind =]
+theorem length_eq_size_sub_iterVal :
+    it.length = aig.size - (aig.iterVal it).idx := by
+  induction it using Std.Iter.inductSteps with | step it ihy _ =>
+  rw [Std.Iter.length_eq_match_step]
+  split <;> grind
+
+grind_pattern length_eq_size_sub_iterVal => it.length, aig.size - (aig.iterVal it).idx
+
+@[simp]
+theorem length_done (h : it.IsPlausibleStep .done) :
+    it.length = 0 := by
+  grind
+
+grind_pattern length_done => it.IsPlausibleStep .done, it.length
+
+@[simp]
+theorem length_zero_done (h : it.length = 0) :
+    it.step.val = .done := by
+  grind
+
+grind_pattern length_zero_done => it.length, it.step
+
+@[simp]
+theorem length_yield (h : it.IsPlausibleStep (.yield it' out)) :
+    it'.length = it.length - 1 := by
+  grind
+
+@[simp]
+theorem length_yield_gt_zero (h : it.IsPlausibleStep (.yield it' out)) :
+    it.length > 0 := by
+  grind
+
+@[simp, grind .]
+theorem length_yield' (h : it.IsPlausibleStep (.yield it' out)) :
+    it'.length + 1 = it.length := by
+  grind
+
+@[simp, grind .]
+theorem length_le_size :
+    it.length ≤ aig.nodes.size := by
+  grind
+
+@[simp, grind →]
+theorem done_eq (h : it.IsPlausibleStep .done) :
+    it = aig.iterEnd := by
+  grind
+
+@[simp, grind .]
+theorem iterVal_yield (h : it.IsPlausibleStep  (.yield it' out)) :
+    aig.iterVal it' = aig.iterVal it + 1 := by
+  grind
+
+@[simp, grind →]
+theorem out_yield (h : it.IsPlausibleStep (.yield it' out)) :
+    out = aig.iterVal it := by
+  grind
+
+@[simp, grind .]
+theorem iterVal_yield_mem_nodes (h : it.IsPlausibleStep (.yield it' out)) :
+    (aig.iterVal it) ∈ aig.nodes := by
+  grind
+
+@[local grind =]
+theorem toList_eq_ofFn :
+    it.toList = List.ofFn (fun (n : Fin it.length) => aig.iterVal it + n.val) := by
+  induction it using Std.Iter.inductSteps with | step it ihy _ =>
+  rw [Std.Iter.toList_eq_match_step] 
+  apply List.ext_getElem <;> split <;> grind
+
+@[simp]
+theorem toList_done (h : it.IsPlausibleStep .done) :
+    it.toList = [] := by
+  grind
+
+grind_pattern toList_done => it.IsPlausibleStep .done, it.toList
+
+theorem toList_yield (h : it.IsPlausibleStep (.yield it' out)) :
+    it.toList = out :: it'.toList := by
+  induction h : it.toList with
+  | nil => grind [List.ofFn_eq_nil_iff]
+  | cons out' tail ih =>
+    rw [Std.Iter.toList_eq_match_step]
+    apply List.ext_getElem <;> split <;> grind
+
+grind_pattern toList_yield => it.IsPlausibleStep (.yield it' out), it.toList
+
+@[simp, grind =]
+theorem step_iterEnd :
+    aig.iterEnd.step.val = .done := by
+  grind
+
+@[simp, grind .]
+theorem iterVal_le_nextVar :
+    aig.iterVal it ≤ aig.nextVar := by
+  grind
+
+@[simp, grind =]
+theorem mem_nodes_iff_not_iterEnd :
+    (aig.iterVal it) ∈ aig.nodes ↔ it ≠ aig.iterEnd := by
+  grind
+
+end VarIter
+
+attribute [local simp, local grind =] VarIter.iterVal_eq
+
+@[simp, grind =]
+theorem iterVal_iter :
+    aig.iterVal aig.iter = .constant := by
+  grind [iter, iterVal]
+
+@[simp, grind =]
+theorem iterVal_iterEnd :
+    aig.iterVal aig.iterEnd = aig.nextVar := by
+  grind [iterEnd, iterVal]
+
+@[simp, grind =]
+theorem length_iter :
+    aig.iter.length = aig.nodes.size := by
+  grind [VarIter.length_eq_size_sub_iterVal]
+
+@[simp, grind =]
+theorem length_toList_iter :
+    aig.iter.toList.length = aig.nodes.size := by
+  grind
+
+@[grind =]
+theorem toList_iter :
+    aig.iter.toList = List.ofFn (fun (n : Fin aig.size) => .ofIdx n) := by
+  apply List.ext_getElem
+  · grind
+  · grind [iter, VarIter.toList_eq_ofFn]
+
+@[simp, grind =]
+theorem mem_iter {var : Var} :
+    var ∈ aig.iter.toList ↔ var ∈ aig.nodes := by
+  simp only [toList_iter, List.mem_ofFn]
+  constructor
+  · grind [Var.validIn]
+  · intro h
+    exists ⟨var.idx, by grind⟩
+
+@[simp, grind .]
+theorem nodup_toList_iter :
+    aig.iter.toList.Nodup := by
+  grind [iter, List.pairwise_iff_getElem]
+
+theorem distinct_toList_iter {idx idx' : Nat} (h : idx < aig.iter.length) (h' : idx' < aig.iter.length)
+    (diff : idx ≠ idx') :
+      aig.iter.toList[idx] ≠ aig.iter.toList[idx'] := by
+  grind [@nodup_toList_iter aig, List.pairwise_iff_getElem]
+
+grind_pattern distinct_toList_iter => aig.iter.toList[idx], aig.iter.toList[idx'] where
+  idx =/= idx'
+
+theorem Perm_iter_iff {aig aig' : Aig} :
+    aig'.iter.toList.Perm aig.iter.toList ↔
+    ∀ (var : Var), var ∈ aig'.nodes ↔ var ∈ aig.nodes := by
+  constructor
+  · grind [=_ mem_iter, List.Perm.mem_iff]
+  · grind [List.Nodup.count]
+
+theorem size_nodes_eq_of_mem_nodes_eq {aig aig' : Aig} (h : ∀ (var : Var), var ∈ aig'.nodes ↔ var ∈ aig.nodes) :
+    aig'.nodes.size = aig.nodes.size := by
+  grind [=_ length_toList_iter, Perm_iter_iff, List.Perm.length_eq]
+
+@[simp]
+theorem toList_iter_prefix_mono {old new : Aig} (mono : old ≤ new):
+    old.iter.toList <+: new.iter.toList := by
+  grind [List.prefix_iff_getElem]
+
+end iter
+
+/-
+  `inputsIter`.
+-/
+section inputsIter
+attribute [local simp, local grind] inputsIter
+
+@[simp, grind =]
+theorem length_inputsiter :
+    aig.inputsIter.length = aig.inputs.size := by
+  grind [inputs]
+
+@[simp, grind =]
+theorem length_toList_inputsIter :
+    aig.inputsIter.toList.length = aig.inputs.size := by
+  grind
+
+@[simp, grind =]
+theorem mem_inputsIter {idx : InputIdx} :
+    idx ∈ aig.inputsIter.toList ↔ idx ∈ aig.inputs := by
+  grind [inputs]
+
+@[simp, grind .]
+theorem nodup_inputsIter :
+    aig.inputsIter.toList.Nodup := by
+  grind [List.pairwise_iff_getElem]
+
+theorem distinct_inputsIter {idx idx' : Nat} (h : idx < aig.inputsIter.length) (h' : idx' < aig.inputsIter.length)
+    (diff : idx ≠ idx') :
+      aig.inputsIter.toList[idx] ≠ aig.inputsIter.toList[idx'] := by
+  grind [@nodup_inputsIter aig, List.pairwise_iff_getElem]
+
+grind_pattern distinct_inputsIter => aig.inputsIter.toList[idx], aig.inputsIter.toList[idx'] where
+  idx =/= idx'
+
+theorem Perm_inputsIter_iff {aig aig' : Aig} :
+    aig'.inputsIter.toList.Perm aig.inputsIter.toList ↔
+    ∀ (idx : InputIdx), idx ∈ aig'.inputs ↔ idx ∈ aig.inputs := by
+  constructor
+  · grind [=_ mem_inputsIter, List.Perm.mem_iff]
+  · grind [List.Nodup.count]
+
+theorem size_inputs_eq_of_mem_inputs_eq {aig aig' : Aig} (h : ∀ (idx : InputIdx), idx ∈ aig'.inputs ↔ idx ∈ aig.inputs) :
+    aig'.inputs.size = aig.inputs.size := by
+  grind [=_ length_toList_inputsIter, Perm_inputsIter_iff, List.Perm.length_eq]
+
+@[simp]
+theorem toList_inputsIter_subset_mono {old new : Aig} (mono : old ≤ new) :
+    old.inputsIter.toList ⊆ new.inputsIter.toList := by
+  grind
+
+end inputsIter
+
+/-
+  `latchesIter`.
+-/
+section latchesIter
+attribute [local simp, local grind] latchesIter
+
+@[simp, grind =]
+theorem length_latchesiter :
+    aig.latchesIter.length = aig.latches.size := by
+  grind [latches]
+
+@[simp, grind =]
+theorem length_toList_latchesIter :
+    aig.latchesIter.toList.length = aig.latches.size := by
+  grind
+
+@[simp, grind =]
+theorem mem_latchesIter {idx : LatchIdx} :
+    idx ∈ aig.latchesIter.toList ↔ idx ∈ aig.latches := by
+  grind [latches]
+
+@[simp, grind .]
+theorem nodup_latchesIter :
+    aig.latchesIter.toList.Nodup := by
+  grind [List.pairwise_iff_getElem]
+
+theorem distinct_latchesIter {idx idx' : Nat} (h : idx < aig.latchesIter.length) (h' : idx' < aig.latchesIter.length)
+    (diff : idx ≠ idx') :
+      aig.latchesIter.toList[idx] ≠ aig.latchesIter.toList[idx'] := by
+  grind [@nodup_latchesIter aig, List.pairwise_iff_getElem]
+
+grind_pattern distinct_latchesIter => aig.latchesIter.toList[idx], aig.latchesIter.toList[idx'] where
+  idx =/= idx'
+
+theorem Perm_latchesIter_iff {aig aig' : Aig} :
+    aig'.latchesIter.toList.Perm aig.latchesIter.toList ↔
+    ∀ (idx : LatchIdx), idx ∈ aig'.latches ↔ idx ∈ aig.latches := by
+  constructor
+  · grind [=_ mem_latchesIter, List.Perm.mem_iff]
+  · grind [List.Nodup.count]
+
+theorem size_latches_eq_of_mem_latches_eq {aig aig' : Aig} (h : ∀ (idx : LatchIdx), idx ∈ aig'.latches ↔ idx ∈ aig.latches) :
+    aig'.latches.size = aig.latches.size := by
+  grind [=_ length_toList_latchesIter, Perm_latchesIter_iff, List.Perm.length_eq]
+
+@[simp]
+theorem toList_latchesIter_subset_mono {old new : Aig} (mono : old ≤ new) :
+    old.latchesIter.toList ⊆ new.latchesIter.toList := by
+  grind
+
+end latchesIter
+
+end Valaig.Aig
